coq/theories/imp2asm/ImpToASMCodegen.v
@@ -5,6 +5,7 @@ Require Import impboot.utils.AppList.
 Require Import coqutil.Word.Interface.
 Require Import ZArith.
 Require Import FunInd.
+Require Import Ascii.
 
 Open Scope app_list_scope.
 
@@ -14,7 +15,7 @@ Notation v_stack := (list (option name)).
 Notation f_lookup := (list (name * nat)).
 
 (* Generates the initialization code for execution *)
-Definition init (k : nat) : asm :=
+Definition init (k: nat): asm :=
   [
     (*  0 *) ASMSyntax.Const RAX (word.of_Z (Z.of_nat 0));
     (*  1 *) ASMSyntax.Const R12 (word.of_Z (Z.of_nat 16));
@@ -25,34 +26,92 @@ Definition init (k : nat) : asm :=
     (*  4 *) ASMSyntax.Const RDI (word.of_Z (Z.of_nat 0));
     (*  5 *) ASMSyntax.Exit;
     (* alloc routine starts here: *)
-    (*  6 *) ASMSyntax.Comment "malloc";
+    (*  6 *) ASMSyntax.Comment ["m"; "a"; "l"; "l"; "o"; "c"];
     (*  7 *) ASMSyntax.Mov RDI RAX;
     (*  8 *) ASMSyntax.Mov RAX R14;
     (*  9 *) ASMSyntax.Add R14 RDI;
     (* 10 *) ASMSyntax.Jump (ASMSyntax.Less R15 R14) 14;
-    (* 11 *) ASMSyntax.Comment "noop";
+    (* 11 *) ASMSyntax.Comment ["n"; "o"; "o"; "p"];
     (* 12 *) ASMSyntax.Ret;
     (* give up: *)
-    (* 13 *) ASMSyntax.Comment "exit 4"; (* Internal error – OOM or compiler limitation *)
+    (* 13 *) ASMSyntax.Comment ["e"; "x"; "i"; "t"; " "; "4"]; (* Internal error – OOM or compiler limitation *)
     (* 14 *) ASMSyntax.Push R15; (* align stack *)
     (* 15 *) ASMSyntax.Const RDI (word.of_Z (Z.of_nat 4));
     (* 16 *) ASMSyntax.Exit;
     (* abort: *)
-    (* 17 *) ASMSyntax.Comment "exit 1"; (* Internal error – OOM or compiler limitation *)
+    (* 17 *) ASMSyntax.Comment ["e"; "x"; "i"; "t"; " "; "1"]; (* Internal error – OOM or compiler limitation *)
     (* 18 *) ASMSyntax.Push R15; (* align stack *)
     (* 19 *) ASMSyntax.Const RDI (word.of_Z (Z.of_nat 1));
     (* 20 *) ASMSyntax.Exit
-  ].
+  ]%char.
 
-Definition AllocLoc : nat := 7.
+Definition AllocLoc: nat := 7.
 
-Function even_len (xs: v_stack): bool :=
+(* START boilerplate *)
+
+Function list_length_v_stack (l: v_stack): nat :=
+  match l with
+  | x :: l => 1 + list_length_v_stack l
+  | [] => 0
+  end.
+
+Function list_length_exp (l: list exp): nat :=
+  match l with
+  | x :: l => 1 + list_length_exp l
+  | [] => 0
+  end.
+
+Function list_length_name (l: list name): nat :=
+  match l with
+  | x :: l => 1 + list_length_name l
+  | [] => 0
+  end.
+
+Function list_append_asm (l1 l2: asm): asm :=
+  match l1 with
+  | x :: l1 => x :: (list_append_asm l1 l2)
+  | [] => l2
+  end.
+
+Function list_append_v_stack (l1 l2: v_stack): v_stack :=
+  match l1 with
+  | x :: l1 => x :: (list_append_v_stack l1 l2)
+  | [] => l2
+  end.
+
+Function list_append_name (l1 l2: list name): list name :=
+  match l1 with
+  | x :: l1 => x :: (list_append_name l1 l2)
+  | [] => l2
+  end.
+
+Function list_length_asm (l: asm): nat :=
+  match l with
+  | x :: l => 1 + list_length_asm l
+  | [] => 0
+  end.
+
+Function flatten_asm (xs: asm_appl): asm :=
+  match xs with
+  | List l => l
+  | Append l1 l2 => list_append_asm (flatten_asm l1) (flatten_asm l2)
+  end.
+
+Function app_list_length_asm (xs: asm_appl): nat :=
+  match xs with
+  | List l => list_length_asm l
+  | Append l1 l2 => app_list_length_asm l1 + app_list_length_asm l2
+  end.
+
+(* END boilerplate *)
+
+Function even_len_v_stack (xs: v_stack): bool :=
   match xs with
   | nil => true
   | _ :: ys =>
     match ys with
     | nil => false
-    | _ :: zs => even_len zs
+    | _ :: zs => even_len_v_stack zs
     end
   end.
 
@@ -66,13 +125,13 @@ Function even_len_exp (xs: list exp): bool :=
     end
   end.
 
-Function odd_len (xs: v_stack) : bool :=
+Function odd_len_v_stack (xs: v_stack) : bool :=
   match xs with
   | nil => false
   | _ :: ys =>
     match ys with
     | nil => true
-    | _ :: zs => odd_len zs
+    | _ :: zs => odd_len_v_stack zs
     end
   end.
 
@@ -139,14 +198,14 @@ Definition c_assign (n : name) (l : nat) (vs : v_stack) : (asm_appl * nat) :=
 (*
   RAX := RAX + top_of_stack
 *)
-Definition c_add (vs : v_stack) : asm_appl :=
+Definition c_add: asm_appl :=
   List [ ASMSyntax.Pop RDI;
     ASMSyntax.Add RAX RDI ].
 
 (*
   RAX := top_of_stack - RAX (or 0 if the result would be negative)
 *)
-Definition c_sub (l : nat) : asm_appl :=
+Definition c_sub: asm_appl :=
   List [ ASMSyntax.Pop RDI;
     ASMSyntax.Sub RDI RAX;
     ASMSyntax.Mov RAX RDI ].
@@ -155,14 +214,14 @@ Definition c_sub (l : nat) : asm_appl :=
   RAX := RAX / top_of_stack
   RDX := RAX % top_of_stack
 *)
-Definition c_div : asm_appl :=
+Definition c_div: asm_appl :=
   List [ ASMSyntax.Mov RDI RAX;
     ASMSyntax.Pop RAX;
     ASMSyntax.Const RDX (word.of_Z (Z.of_nat 0));
     ASMSyntax.Div RDI ].
 
-Definition c_alloc (vs : v_stack) : asm_appl :=
-  if even_len vs (* stack must be aligned at call *)
+Definition c_alloc (vs: v_stack): asm_appl :=
+  if even_len_v_stack vs (* stack must be aligned at call *)
   then List [Load_RSP RDI 0; ASMSyntax.Call AllocLoc; Pop RDI]
   else List [Pop RDI; ASMSyntax.Call AllocLoc].
 
@@ -171,16 +230,16 @@ the stack to 16-bytes before function calls. If `vs` is even – we have to push
 something to the stack before calling any function. (the first value from the stack is kept in RAX,
 so the actual stack size is odd then)
 *)
-Definition align (needs_alignment : bool) (asm1 : asm_appl) : asm_appl :=
+Definition align (needs_alignment: bool) (asm1: asm_appl): asm_appl :=
   if needs_alignment then (List [Push RAX]) +++ asm1 +++ (List [Pop RDI]) else asm1.
 
-Definition c_read (vs : v_stack) (l : nat) : (asm_appl * nat) :=
-  let/d asm1 := align (even_len vs) (List [ASMSyntax.Push RAX; ASMSyntax.GetChar]) in
-  (asm1, l + app_list_length asm1).
+Definition c_read (vs: v_stack) (l: nat): (asm_appl * nat) :=
+  let/d asm1 := align (even_len_v_stack vs) (List [ASMSyntax.Push RAX; ASMSyntax.GetChar]) in
+  (asm1, l + app_list_length_asm asm1).
 
-Definition c_write (vs : v_stack) (l : nat) : (asm_appl * nat) :=
-  let/d asm1 := align (even_len vs) (List [Mov RDI RAX; ASMSyntax.PutChar; ASMSyntax.Const RAX (word.of_Z (Z.of_nat 0))]) in
-  (asm1, l + app_list_length asm1).
+Definition c_write (vs: v_stack) (l: nat): (asm_appl * nat) :=
+  let/d asm1 := align (even_len_v_stack vs) (List [Mov RDI RAX; ASMSyntax.PutChar; ASMSyntax.Const RAX (word.of_Z (Z.of_nat 0))]) in
+  (asm1, l + app_list_length_asm asm1).
 
 (*
   input : RAX, top_of_stack
@@ -188,7 +247,7 @@ Definition c_write (vs : v_stack) (l : nat) : (asm_appl * nat) :=
   i.e.
   load (into)RAX (RAX + top of stack) 0w
 *)
-Definition c_load : asm_appl :=
+Definition c_load: asm_appl :=
   List [ ASMSyntax.Pop RDI;
     ASMSyntax.Add RDI RAX;
     ASMSyntax.Load RAX RDI (word.of_Z (Z.of_nat 0)) ].
@@ -197,34 +256,34 @@ Definition c_load : asm_appl :=
   input : RAX, top_of_stack, snd_top_of_stack
   snd_top_of_stack[top_of_stack] := RAX
 *)
-Definition c_store : asm_appl :=
+Definition c_store: asm_appl :=
   List [ ASMSyntax.Pop RDI;
     ASMSyntax.Pop RDX;
     ASMSyntax.Add RDI RDX;
     ASMSyntax.Store RAX RDI (word.of_Z (Z.of_nat 0)) ].
 
-Fixpoint c_exp (e : exp) (l : nat) (vs : v_stack) : asm_appl * nat :=
+Fixpoint c_exp (e: exp) (l: nat) (vs: v_stack): asm_appl * nat :=
   match e with
   | Var n => c_var n l vs
   | Const n => c_const n l
   | Add e1 e2 =>
-      let/d '(asm1, l1) := c_exp e1 l vs in
-      let/d '(asm2, l2) := c_exp e2 l1 (None :: vs) in
-      let/d c_add_asm := c_add (None :: None :: vs) in
-      (asm1 +++ asm2 +++ c_add_asm, l2 + app_list_length c_add_asm)
+    let/d '(asm1, l1) := c_exp e1 l vs in
+    let/d '(asm2, l2) := c_exp e2 l1 (None :: vs) in
+    let/d c_add_asm := c_add in
+    (asm1 +++ asm2 +++ c_add_asm, l2 + app_list_length_asm c_add_asm)
   | Sub e1 e2 =>
-      let/d '(asm1, l1) := c_exp e1 l vs in
-      let/d '(asm2, l2) := c_exp e2 l1 (None :: vs) in
-      let/d c_sub_asm := c_sub l2 in
-      (asm1 +++ asm2 +++ c_sub_asm, l2 + app_list_length c_sub_asm)
+    let/d '(asm1, l1) := c_exp e1 l vs in
+    let/d '(asm2, l2) := c_exp e2 l1 (None :: vs) in
+    let/d c_sub_asm := c_sub in
+    (asm1 +++ asm2 +++ c_sub_asm, l2 + app_list_length_asm c_sub_asm)
   | Div e1 e2 =>
-      let/d '(asm1, l1) := c_exp e1 l vs in
-      let/d '(asm2, l2) := c_exp e2 l1 (None :: vs) in
-      (asm1 +++ asm2 +++ c_div, l2 + app_list_length c_div)
+    let/d '(asm1, l1) := c_exp e1 l vs in
+    let/d '(asm2, l2) := c_exp e2 l1 (None :: vs) in
+    (asm1 +++ asm2 +++ c_div, l2 + app_list_length_asm c_div)
   | Read e1 e2 =>
-      let/d '(asm1, l1) := c_exp e1 l vs in
-      let/d '(asm2, l2) := c_exp e2 l1 (None :: vs) in
-      (asm1 +++ asm2 +++ c_load, l2 + app_list_length c_load)
+    let/d '(asm1, l1) := c_exp e1 l vs in
+    let/d '(asm2, l2) := c_exp e2 l1 (None :: vs) in
+    (asm1 +++ asm2 +++ c_load, l2 + app_list_length_asm c_load)
   end.
 
 Fixpoint c_exps (es: list exp) (l: nat) (vs: v_stack): asm_appl * nat :=
@@ -241,8 +300,8 @@ Fixpoint c_exps (es: list exp) (l: nat) (vs: v_stack): asm_appl * nat :=
 *)
 Definition c_cmp (c : cmp) : cond :=
   match c with
-    | Less => ASMSyntax.Less RDI RBX
-    | Equal => ASMSyntax.Equal RDI RBX
+  | Less => ASMSyntax.Less RDI RBX
+  | Equal => ASMSyntax.Equal RDI RBX
   end.
 
 Fixpoint c_test_jump (t: test) (pos_label: nat) (neg_label: nat)
@@ -254,7 +313,7 @@ Fixpoint c_test_jump (t: test) (pos_label: nat) (neg_label: nat)
     let/d c_cmp_asm := List [Mov RBX RAX; Pop RDI; Pop RAX;
       ASMSyntax.Jump (c_cmp c) pos_label;
       ASMSyntax.Jump Always neg_label] in
-    (asm1 +++ asm2 +++ c_cmp_asm, l2 + app_list_length c_cmp_asm)
+    (asm1 +++ asm2 +++ c_cmp_asm, l2 + app_list_length_asm c_cmp_asm)
   | And t1 t2 =>
     let/d '(asm1, l1) := c_test_jump t1 (l + 1) neg_label (l + 2) vs in
     let/d '(asm2, l2) := c_test_jump t2 pos_label neg_label l1 vs in
@@ -280,20 +339,23 @@ Function lookup (fs: f_lookup) (n: nat): nat :=
   end.
 
 (* Drop the current stack frame - elements corresponding to `vs` *)
-Definition make_ret (vs : v_stack) (l : nat) : asm_appl * nat :=
-  (List [Add_RSP (List.length vs); Ret], l + 2).
+Definition make_ret (vs: v_stack) (l: nat): asm_appl * nat :=
+  (List [Add_RSP (list_length_v_stack vs); Ret], l + 2).
+
+(* Should this be different than just give_up and we prove that this never happens *)
+(* Maybe just don't include this in the `ec = _ \/ ec = _` post condition *)
 
 (* Store the variables from the stack in the registers, so that they can be
 passed to the function call *)
-Definition c_pops (xs : list exp) (vs : v_stack) : asm_appl :=
-  let/d k := List.length xs in
+Definition c_pops (xs: list exp) (vs: v_stack): asm_appl :=
+  let/d k := list_length_exp xs in
   if k =? 0 then List [Push RAX] else
   if k =? 1 then List [] else
   if k =? 2 then List [Pop RDI] else
   if k =? 3 then List [Pop RDI; Pop RDX] else
   if k =? 4 then List [Pop RDI; Pop RDX; Pop RBX] else
   if k =? 5 then List [Pop RDI; Pop RDX; Pop RBX; Pop RBP] else
-  List [Jump Always (give_up (xorb (negb (even_len_exp xs)) (even_len vs)))].
+  List [Jump Always (give_up (negb (Bool.eqb (even_len_exp xs) (even_len_v_stack vs))))].
 
 (** Builds a stack representation for parameters of a function *)
 Function call_v_stack (xs: list name) (acc: v_stack): v_stack :=
@@ -304,8 +366,8 @@ Function call_v_stack (xs: list name) (acc: v_stack): v_stack :=
 
 (** Push a list of variables onto the stack *)
 Definition c_pushes (v_names: list name) (l: nat): (asm_appl * v_stack * nat) :=
-  let/d k := List.length v_names in
-  let/d e := call_v_stack v_names [] in
+  let/d k := list_length_name v_names in
+  let/d e := call_v_stack v_names (@nil (option name)) in
   if k =? 0 then (List [], [None], l) else
   if k =? 1 then (List [], e, l) else
   if k =? 2 then (List [Push RDI], e, l + 1) else
@@ -314,11 +376,10 @@ Definition c_pushes (v_names: list name) (l: nat): (asm_appl * v_stack * nat) :=
   (List [Push RBP; Push RBX; Push RDX; Push RDI], e, l + 4).
 
 (* Call the given function, passing the arguments in registers*)
-Definition c_call (vs: v_stack) (target: nat)
-  (xs: list exp) (l: nat): asm_appl * nat :=
+Definition c_call (vs: v_stack) (target: nat) (xs: list exp) (l: nat): asm_appl * nat :=
   let/d asm_pops := c_pops xs vs in
-  let/d asm1 := align (even_len vs) (List [ASMSyntax.Call target]) in
-  (asm_pops +++ asm1, l + app_list_length asm_pops + app_list_length asm1).
+  let/d asm1 := align (even_len_v_stack vs) (List [ASMSyntax.Call target]) in
+  (asm_pops +++ asm1, l + app_list_length_asm asm_pops + app_list_length_asm asm1).
 
 Fixpoint c_cmd (c: cmd) (l: nat) (fs: f_lookup) (vs: v_stack): (asm_appl * nat) :=
   match c with
@@ -336,7 +397,7 @@ Fixpoint c_cmd (c: cmd) (l: nat) (fs: f_lookup) (vs: v_stack): (asm_appl * nat) 
     let/d '(asm2, l2) := c_exp e l1 vs in
     let/d '(asm3, l3) := c_exp e' l2 (None :: vs) in
     let/d asm4 := c_store in
-    (asm1 +++ asm2 +++ asm3 +++ asm4, l3 + app_list_length asm4)
+    (asm1 +++ asm2 +++ asm3 +++ asm4, l3 + app_list_length_asm asm4)
   | If t c1 c2 =>
     let/d '(asm1, l1) := c_test_jump t (l + 1) (l + 2) (l + 3) vs in
     let/d '(asm2, l2) := c_cmd c1 l1 fs vs in
@@ -369,7 +430,7 @@ Fixpoint c_cmd (c: cmd) (l: nat) (fs: f_lookup) (vs: v_stack): (asm_appl * nat) 
   | Alloc n e =>
     let/d '(asm1, l1) := c_exp e l vs in
     let/d asm2 := c_alloc vs in
-    let/d '(asm3, l3) := c_assign n (l1 + app_list_length asm2) vs in
+    let/d '(asm3, l3) := c_assign n (l1 + app_list_length_asm asm2) vs in
     (asm1 +++ asm2 +++ asm3, l3)
   | GetChar n =>
     let/d '(asm1, l1) := c_read vs l in
@@ -380,16 +441,16 @@ Fixpoint c_cmd (c: cmd) (l: nat) (fs: f_lookup) (vs: v_stack): (asm_appl * nat) 
     let/d '(asm2, l2) := c_write vs l1 in
     (asm1 +++ asm2, l2)
   | Abort =>
-    (List [Jump Always (abort (odd_len vs))], l+1)
+    (List [Jump Always (abort (odd_len_v_stack vs))], l+1)
   end.
 
 Function all_binders (body: cmd): list name :=
   match body with
   | Skip => []
-  | Seq c1 c2 => all_binders c1 ++ all_binders c2
+  | Seq c1 c2 => list_append_name (all_binders c1) (all_binders c2)
   | Assign n e => [n]
   | Update a e e' => []
-  | If t c1 c2 => all_binders c1 ++ all_binders c2
+  | If t c1 c2 => list_append_name (all_binders c1) (all_binders c2)
   | While tst body => all_binders body
   | Call n f es => [n]
   | Return e => []
@@ -402,7 +463,9 @@ Function all_binders (body: cmd): list name :=
 Function names_contain (l: list name) (a: name): bool :=
   match l with
   | nil => false
-  | x :: l => (x =? a) || names_contain l a
+  | x :: l =>
+    if (x =? a) then true
+    else names_contain l a
   end.
 
 Fixpoint names_unique (l: list name) (acc: list name): list name :=
@@ -428,21 +491,32 @@ Definition c_fundef (fundef: func) (l: nat) (fs: f_lookup): (asm_appl * nat) :=
     let/d '(asm0, vs0, l0) := c_pushes v_names l in
     let/d binders := unique_binders body in
     let/d vs_binders := make_vs_from_binders binders in
-    let/d asm1 := List [Sub_RSP (List.length vs_binders)] in
-    let/d '(asm2, l2) := c_cmd body (l0 + 1) fs (vs_binders ++ vs0) in
+    let/d asm1 := List [Sub_RSP (list_length_v_stack vs_binders)] in
+    let/d '(asm2, l2) := c_cmd body (l0 + 1) fs (list_append_v_stack vs_binders vs0) in
     (asm0 +++ asm1 +++ asm2, l2)
   end.
 
 (* TODO(kπ) termination is unobvious to Coq, super unimportant function, hacked for now *)
 (* Converts a numeric name to a string representation *)
-Fail Function name2str (n: nat) (acc: string): string :=
+Fail Function name2str (n: nat) (acc: list ascii): list ascii :=
   if n =? 0 then
     acc
   else
-    name2str (n / 256) (String (ascii_of_nat (n mod 256)) acc).
+    name2str (n / 256) (String (ascii_of_N (N_of_nat (n mod 256))) acc).
 
-Definition name2str (n: nat) (acc: string): string :=
-  String (ascii_of_nat (n mod 256)) acc.
+(* TODO: mod? *)
+Definition name2str (n: nat) (acc: list ascii): list ascii :=
+  (ascii_of_N (N_of_nat (n mod 256))) :: acc.
+
+Definition get_funcs (p: prog): list func :=
+  match p with
+  | Program funcs => funcs
+  end.
+
+Definition name_of_func (f: func) : name :=
+  match f with
+  | Func n _ _ => n
+  end.
 
 (* Compiles a list of function declarations into assembly instructions *)
 Fixpoint c_fundefs (ds: list func) (l: nat) (fs: f_lookup): (asm_appl * list (name * nat) * nat) :=
@@ -450,17 +524,25 @@ Fixpoint c_fundefs (ds: list func) (l: nat) (fs: f_lookup): (asm_appl * list (na
   | [] => (List [], fs, l)
   | d :: ds' =>
     let/d fname := name_of_func d in
-    let/d comment := List [Comment (name2str fname "")] in
+    let/d comment := List [Comment (name2str fname [])] in
     let/d '(c1, l1) := c_fundef d (l + 1) fs in
     let/d '(c2, fs', l2) := c_fundefs ds' l1 fs in
     (comment +++ c1 +++ c2, (fname, l + 1) :: fs', l2)
   end.
 
+Fixpoint fun_name_of_string (str: string): name :=
+  match str with
+  | EmptyString => 0
+  | String c s => (nat_of_ascii c) * 256 + fun_name_of_string s
+  end.
+
+(* Compute (fun_name_of_string "main"). *)
+
 (* Generates the complete assembly code for a given program *)
 Definition codegen (prog : prog) : asm :=
   let/d funs := get_funcs prog in
-  let/d init_l := app_list_length (List (init 0)) in
+  let/d init_l := app_list_length_asm (List (init 0)) in
   let/d '(_, fs, _) := c_fundefs funs init_l [] in
   let/d '(asm1, _, _) := c_fundefs funs init_l fs in
   let/d main_l := lookup fs (fun_name_of_string "main") in
-  flatten ((List (init main_l)) +++ asm1).
+  flatten_asm ((List (init main_l)) +++ asm1).
