coq/theories/imperative/ImpSyntax.v
@@ -18,46 +18,15 @@ Inductive exp : Type :=
 | Div (e1: exp) (e2: exp)   (*  word division        *)
 | Read (e1: exp) (e2: exp). (*  read memory:  e[e']  *)
 
-Definition exp_CASE {A} (e: exp)
-  (vcase: name -> A) (ccase: word64 -> A)
-  (acase: exp -> exp -> A) (scase: exp -> exp -> A)
-  (dcase: exp -> exp -> A) (rcase: exp -> exp -> A) : A :=
-  match e with
-  | Var n => vcase n
-  | Const n => ccase n
-  | Add e1 e2 => acase e1 e2
-  | Sub e1 e2 => scase e1 e2
-  | Div e1 e2 => dcase e1 e2
-  | Read e1 e2 => rcase e1 e2
-  end.
-
 Inductive cmp : Type :=
 | Less
 | Equal.
-
-Definition cmp_CASE {A} (c: cmp) (less: A) (equal: A) : A :=
-  match c with
-  | Less => less
-  | Equal => equal
-  end.
 
 Inductive test : Type :=
 | Test (c: cmp) (e1: exp) (e2: exp) (* e1 `cmp` e2 *)
 | And (t1: test) (t2: test)         (* t1 && t2 *)
 | Or (t1: test) (t2: test)          (* t1 || t2 *)
 | Not (t: test).                    (* !t *)
-
-Definition test_CASE {A} (t: test)
-  (tcase: cmp -> exp -> exp -> A)
-  (acase: test -> test -> A)
-  (ocase: test -> test -> A)
-  (ncase: test -> A) : A :=
-  match t with
-  | Test c e1 e2 => tcase c e1 e2
-  | And t1 t2 => acase t1 t2
-  | Or t1 t2 => ocase t1 t2
-  | Not t => ncase t
-  end.
 
 Inductive cmd : Type :=
 | Skip
@@ -73,59 +42,11 @@ Inductive cmd : Type :=
 | PutChar (e: exp)                            (*  putchar(e)              *)
 | Abort.                                      (*  exit(1)                 *)
 
-Definition cmd_CASE {A} (c: cmd)
-  (skcase: A)
-  (scase: cmd -> cmd -> A)
-  (acase: name -> exp -> A)
-  (ucase: exp -> exp -> exp -> A)
-  (icase: test -> cmd -> cmd -> A)
-  (wcase: test -> cmd -> A)
-  (ccase: name -> name -> list exp -> A)
-  (rcase: exp -> A)
-  (acase': name -> exp -> A)
-  (gcase: name -> A)
-  (pcase: exp -> A)
-  (abcase: A) : A :=
-  match c with
-  | Skip => skcase
-  | Seq c1 c2 => scase c1 c2
-  | Assign n e => acase n e
-  | Update a e e' => ucase a e e'
-  | If t c1 c2 => icase t c1 c2
-  | While t c => wcase t c
-  | Call n f es => ccase n f es
-  | Return e => rcase e
-  | Alloc n e => acase' n e
-  | GetChar n => gcase n
-  | PutChar e => pcase e
-  | Abort => abcase
-  end.
-
 Inductive func : Type :=
 | Func (n: name) (params: list name) (body: cmd). (* func name, formal params, body *)
 
-Definition func_CASE {A} (f: func) (fcase: name -> list name -> cmd -> A) : A :=
-  match f with
-  | Func n params body => fcase n params body
-  end.
-
 Inductive prog : Type :=
 | Program (funcs: list func). (* a complete program is a list of function definitions *)
-
-Definition prog_CASE {A} (p: prog) (fcase: list func -> A) : A :=
-  match p with
-  | Program funcs => fcase funcs
-  end.
-
-Definition get_funcs (p: prog) : list func :=
-  match p with
-  | Program funcs => funcs
-  end.
-
-Definition name_of_func (f: func) : name :=
-  match f with
-  | Func n _ _ => n
-  end.
 
 Fixpoint fun_name_of_string (str: string): name :=
   match str with
