coq/theories/utils/AppList.v
@@ -1,18 +1,18 @@
-Inductive app_list {A : Type} : Type :=
+Inductive app_list {A: Type}: Type :=
 | List : list A -> app_list
 | Append : app_list -> app_list -> app_list.
-Arguments app_list : clear implicits.
+Arguments app_list: clear implicits.
 
 Declare Scope app_list_scope.
-Notation "xs +++ ys" := (Append xs ys) (right associativity, at level 60) : app_list_scope.
+Notation "xs +++ ys" := (Append xs ys) (right associativity, at level 60): app_list_scope.
 
-Fixpoint flatten {A : Type} (xs : app_list A) : list A :=
+Fixpoint flatten {A: Type} (xs: app_list A): list A :=
   match xs with
   | List l => l
   | Append l1 l2 => flatten l1 ++ flatten l2
   end.
 
-Fixpoint app_list_length {A : Type} (xs : app_list A) : nat :=
+Fixpoint app_list_length {A: Type} (xs: app_list A): nat :=
   match xs with
   | List l => length l
   | Append l1 l2 => app_list_length l1 + app_list_length l2
